common/SmallstepSafe.v
@@ -1,0 +1,183 @@
+Require Import Relations.
+Require Import Wellfounded.
+Require Import Coqlib.
+Require Import Events.
+Require Import Globalenvs.
+Require Import LanguageInterface.
+Require Import Integers.
+Require Import Smallstep.
+
+Set Implicit Arguments.
+
+
+(** * Forward simulation with the progress property and the preservation of UB *)
+
+(* It means that the compilation satisfying this simulation cannot
+utilize the UB to optimize the program *)
+
+Section FSIM_WITH_2P.
+
+Context {liA1 liA2} (ccA: callconv liA1 liA2).
+Context {liB1 liB2} (ccB: callconv liB1 liB2).
+Context (se1 se2: Genv.symtbl) (wB: ccworld ccB).
+Context {state1 state2: Type}.
+
+(** Here we combine the progress property and UB preservation property
+into one definition for convenience. But they should be orthogonal
+concepts and located in two definitions in principal. For example,
+some compilation pass may compile UB to DB (defined behavior) and also
+preserve certain UB (such as memory error state). *)
+
+Record fsimp_properties (L1: lts liA1 liB1 state1) (L2: lts liA2 liB2 state2) (index: Type)
+                       (order: index -> index -> Prop)
+                       (match_states: index -> state1 -> state2 -> Prop)
+                       (err_state1: state1 -> Prop) (err_state2: state2 -> Prop): Prop := {
+    fsimp_prop:
+    fsim_properties ccA ccB se1 se2 wB L1 L2
+      index order match_states;
+
+    fsimp_initial_progress: forall q1 q2 s2,
+      match_query ccB wB q1 q2 ->
+      initial_state L2 q2 s2 ->
+      exists s1, initial_state L1 q1 s1;
+
+    (** FIXME: this property may be not correct (but it can be proved
+    in RustIRgen?) *)
+    fsimp_external_progress: forall i s1 s2 s2' wA r1 r2,
+      match_states i s1 s2 ->
+      match_reply ccA wA r1 r2 -> 
+      after_external L2 s2 r2 s2' ->
+      exists s1', after_external L1 s1 r1 s1';
+    
+    fsimp_progress: forall i s1 s2,
+      match_states i s1 s2 -> safe L2 s2 ->
+      (exists r, final_state L1 s1 r)
+      \/ (exists q, at_external L1 s1 q)
+      \/ (exists t, exists s1', Step L1 s1 t s1');
+    
+    fsimp_err_preservation: forall i s1 s2,
+      match_states i s1 s2 ->
+      err_state1 s1 ->
+      (* The execution of L2 cannot emit event *)
+      exists s2', Star L2 s2 E0 s2'
+             /\ err_state2 s2';
+  }.
+
+
+End FSIM_WITH_2P.
+
+Arguments fsimp_properties {_ _} _ {_ _} _ _ _ _ {_ _} L1 L2 index order match_states err_state1 err_state2.
+
+(* The error states should be transparent *)
+Record fsimp_components {liA1 liA2} (ccA: callconv liA1 liA2) {liB1 liB2} ccB L1 L2 err_state1 err_state2 :=
+  Forward_simulation_ppub {
+    fsimp_index: Type;
+    fsimp_order: fsimp_index -> fsimp_index -> Prop;
+    fsimp_match_states: _;
+      
+    fsimp_skel:
+      skel L1 = skel L2;
+    fsimp_lts se1 se2 wB:
+      @match_senv liB1 liB2 ccB wB se1 se2 ->
+      Genv.valid_for (skel L1) se1 ->
+      fsimp_properties ccA ccB se1 se2 wB (activate L1 se1) (activate L2 se2)
+        fsimp_index fsimp_order (fsimp_match_states se1 se2 wB) (err_state1 se1) (err_state2 se2);
+    fsimg_order_wf:
+      well_founded fsimp_order;
+  }.
+
+Arguments Forward_simulation_ppub {_ _ ccA _ _ ccB L1 L2 err_state1 err_state2 fsimp_index}.
+
+(* We can treat error_state as the patch of L1/L2 *)
+Definition forward_simulation_ppub {liA1 liA2} ccA {liB1 liB2} ccB L1 L2 err_state1 err_state2 :=
+  inhabited (@fsimp_components liA1 liA2 ccA liB1 liB2 ccB L1 L2 err_state1 err_state2).
+
+(** Backward simulation with the property of UB preservation  *)
+
+Definition partial_safe {liA liB st} (L: lts liA liB st) (err_state: st -> Prop) (s: st) : Prop :=
+  forall s',
+  Star L s E0 s' ->
+  ((exists r, final_state L s' r)
+  \/ (exists q, at_external L s' q)
+  \/ (exists t, exists s'', Step L s' t s''))
+  \/ err_state s'.
+
+Lemma star_partial_safe:
+  forall {liA liB st} (L: lts liA liB st) err s s',
+  Star L s E0 s' -> partial_safe L err s -> partial_safe L err s'.
+Proof.
+  intros; red; intros. apply H0. eapply star_trans; eauto.
+Qed.
+
+Section BSIM.
+
+Context {liA1 liA2} (ccA: callconv liA1 liA2).
+Context {liB1 liB2} (ccB: callconv liB1 liB2).
+Context (se1 se2: Genv.symtbl) (wB: ccworld ccB).
+Context {state1 state2: Type}.
+
+(** The general form of a backward simulation. *)
+
+Record bsimp_properties (L1 L2: lts _ _ _) (index: Type)
+                       (order: index -> index -> Prop)
+                       (match_states: index -> state1 -> state2 -> Prop)
+                       err_state1 err_state2 : Prop := {
+    bsimp_match_valid_query:
+      forall q1 q2, match_query ccB wB q1 q2 ->
+      valid_query L2 q2 = valid_query L1 q1;
+    bsimp_match_initial_states:
+      forall q1 q2, match_query ccB wB q1 q2 ->
+      bsim_match_cont (rex match_states) (initial_state L1 q1) (initial_state L2 q2);
+    bsimp_match_final_states:
+      forall i s1 s2 r2,
+      match_states i s1 s2 -> partial_safe L1 err_state1 s1 -> final_state L2 s2 r2 ->
+      exists s1' r1, Star L1 s1 E0 s1' /\ final_state L1 s1' r1 /\ match_reply ccB wB r1 r2;
+    bsimp_match_external:
+      forall i s1 s2 q2, match_states i s1 s2 -> partial_safe L1 err_state1 s1 -> at_external L2 s2 q2 ->
+      exists wA s1' q1, Star L1 s1 E0 s1' /\ at_external L1 s1' q1 /\
+      match_query ccA wA q1 q2 /\ match_senv ccA wA se1 se2 /\
+      forall r1 r2, match_reply ccA wA r1 r2 ->
+      bsim_match_cont (rex match_states) (after_external L1 s1' r1) (after_external L2 s2 r2);
+    bsimp_progress:
+      forall i s1 s2,
+      match_states i s1 s2 -> partial_safe L1 err_state1 s1 ->
+      ((exists r, final_state L2 s2 r) \/
+      (exists q, at_external L2 s2 q) \/
+      (exists t, exists s2', Step L2 s2 t s2')) \/
+      err_state2 s2;
+    bsimp_simulation:
+      forall s2 t s2', Step L2 s2 t s2' ->
+      forall i s1, match_states i s1 s2 -> partial_safe L1 err_state1 s1 ->
+      exists i', exists s1',
+         (Plus L1 s1 t s1' \/ (Star L1 s1 t s1' /\ order i' i))
+      /\ match_states i' s1' s2';
+  }.
+
+Arguments bsimp_properties: clear implicits.
+
+End BSIM.
+
+Arguments bsimp_properties {_ _} _ {_ _} _ _ _ _ {_ _} L1 L2 index order match_states err_state1 err_state2.
+
+Record bsimp_components {liA1 liA2} (ccA: callconv liA1 liA2) {liB1 liB2} ccB L1 L2 err_state1 err_state2 :=
+  Backward_simulation_preserve_error {
+    bsimp_index: Type;
+    bsimp_order: bsimp_index -> bsimp_index -> Prop;
+    bsimp_match_states: _;
+
+    bsimp_skel:
+      skel L1 = skel L2;
+    bsimp_lts:
+      forall se1 se2 wB,
+        @match_senv liB1 liB2 ccB wB se1 se2 ->
+        Genv.valid_for (skel L1) se1 ->
+        bsimp_properties ccA ccB se1 se2 wB (activate L1 se1) (activate L2 se2)
+                        bsimp_index bsimp_order (bsimp_match_states se1 se2 wB) (err_state1 se1) (err_state2 se2);
+    bsimp_order_wf:
+      well_founded bsimp_order;
+    }.
+
+Arguments Backward_simulation_preserve_error {_ _ ccA _ _ ccB L1 L2 err_state1 err_state2 bsimp_index}.
+
+Definition backward_simulation_preserve_error {liA1 liA2} ccA {liB1 liB2} ccB L1 L2 err_state1 err_state2 :=
+  inhabited (@bsimp_components liA1 liA2 ccA liB1 liB2 ccB L1 L2 err_state1 err_state2).
